theories/Lang/StImp.v
@@ -1,0 +1,566 @@
+From Coq Require Import
+  Nat
+  Strings.String.
+
+From ExtLib Require Import
+  Structures.Maps
+  Data.Map.FMapAList
+  Data.String.
+
+From TICL Require Import
+  ICTree.Core
+  ICTree.SBisim
+  ICTree.Equ
+  ICTree.Interp.State
+  ICTree.Events.State
+  ICTree.Events.Writer.
+
+From TICL Require Import
+  Logic.Core
+  Logic.Trans
+  ICTree.Logic.AX
+  ICTree.Logic.AF
+  ICTree.Logic.EX
+  ICTree.Logic.EF
+  ICTree.Logic.Bind
+  ICTree.Logic.CanStep
+  ICTree.Logic.State.
+
+Generalizable All Variables.
+
+Import ICtree ICTreeNotations TiclNotations.
+Local Open Scope ticl_scope.
+Local Open Scope ictree_scope.
+Local Open Scope nat_scope.
+
+Generalizable All Variables.
+
+Module StImp.
+  Definition Ctx := alist string nat.
+  Definition Mem := stateE Ctx.
+
+  Definition assert(k: string)(p: nat -> Prop)(m: Ctx): Prop :=
+    match lookup k m with
+    | Some v => p v
+    | None => False
+    end.
+
+  Definition load(k: string)(m: Ctx): nat :=
+    match lookup k m with
+    | Some v => v
+    | None => 0
+    end.
+    
+  Inductive CExp :=
+  | CVar (x: string)
+  | CConst (z: nat)
+  | CAdd (x y: CExp)
+  | CSub (x y: CExp).
+
+  Coercion CVar: string >-> CExp.
+  Coercion CConst: nat >-> CExp.
+  
+  Variant CComp :=
+    | CEq  (l r: CExp)
+    | CLe (l r: CExp)
+    | CLt  (l r: CExp).
+  
+  Inductive CProg :=
+  | CAssgn (x: string) (e: CExp)
+  | CIf (c: CComp) (t: CProg) (e: CProg)
+  | CWhile (c: CComp) (b: CProg) 
+  | CSkip
+  | CSeq (l r: CProg).
+
+  Fixpoint cdenote_exp(e: CExp): ictree Mem nat :=
+    match e with
+    | CVar v => m <- get ;; Ret (load v m)
+    | CConst z => Ret z
+    | CAdd a b =>
+        x <- cdenote_exp a ;;
+        y <- cdenote_exp b ;;
+        Ret (x + y)
+    | CSub a b =>
+        x <- cdenote_exp a ;;
+        y <- cdenote_exp b ;;
+        Ret (x - y)
+    end.
+
+  Definition cdenote_comp(c: CComp): ictree Mem bool :=
+    match c with
+    | CEq a b =>
+        x <- cdenote_exp a ;;
+        y <- cdenote_exp b ;;
+        Ret (x =? y)
+    | CLe a b =>
+        x <- cdenote_exp a ;;
+        y <- cdenote_exp b ;;
+        Ret (x <=? y)
+    | CLt a b =>
+        x <- cdenote_exp a ;;
+        y <- cdenote_exp b ;;
+        Ret (x <? y)
+    end.
+
+  Fixpoint cdenote_prog (s: CProg): ictree Mem unit :=
+    match s with
+    | CAssgn x e =>
+        v <- cdenote_exp e;;
+        m <- get ;;        
+        put (add x v m)
+    | CIf c t e =>
+        bv <- cdenote_comp c ;;
+        if bv then
+          cdenote_prog t
+        else
+          cdenote_prog e
+    | CWhile c b =>       
+        ICtree.iter
+          (fun _ =>
+             cv <- cdenote_comp c ;;
+             if cv then
+               bv <- cdenote_prog b ;;
+               continue
+             else
+               break) tt
+    | CSkip => Ret tt        
+    | CSeq l r =>
+        cdenote_prog l ;;
+        cdenote_prog r
+    end.
+
+  (* Instrumentation of expressions, comparisons and programs *)
+  Definition instr_exp(e: CExp) (ctx: Ctx) : ictreeW Ctx (nat * Ctx) :=
+    instr_stateE (cdenote_exp e) ctx.
+
+  Definition instr_comp(c: CComp) (ctx: Ctx) : ictreeW Ctx (bool * Ctx) :=
+    instr_stateE (cdenote_comp c) ctx.
+    
+  Definition instr_prog(p: CProg) (ctx: Ctx) : ictreeW Ctx (unit * Ctx) :=
+    instr_stateE (cdenote_prog p) ctx.
+  
+  Declare Scope stimp_scope.
+  Local Open Scope stimp_scope.
+  Local Open Scope string_scope.
+  Declare Custom Entry stimp.
+  
+  Notation "[[ e ]]" := e (at level 0, e custom stimp at level 95) : stimp_scope.
+  Notation "( x )" := x (in custom stimp, x at level 99) : stimp_scope.
+  Notation "{ x }" := x (in custom stimp at level 0, x constr): stimp_scope.
+  Notation "x" := x (in custom stimp at level 0, x constr at level 0) : stimp_scope.
+
+  Notation "a + b" := (CAdd a b)
+                        (in custom stimp at level 50, left associativity) : stimp_scope.
+
+  Notation "a - b" := (CSub a b)
+                        (in custom stimp at level 50, left associativity) : stimp_scope.
+
+  Notation "x := c" := (CAssgn x c)
+                         (in custom stimp at level 60, right associativity) : stimp_scope.
+
+  Notation "a =? b" := (CEq a b)
+                         (in custom stimp at level 52, left associativity) : stimp_scope.
+  Notation "a >=? b" := (CLe b a)
+                          (in custom stimp at level 52, left associativity) : stimp_scope.
+  Notation "a >? b" := (CLt b a)
+                         (in custom stimp at level 52, left associativity) : stimp_scope.
+  Notation "a <=? b" := (CLe a b)
+                          (in custom stimp at level 52, left associativity) : stimp_scope.
+  Notation "a <? b" := (CLt a b)
+                         (in custom stimp at level 52, left associativity) : stimp_scope.
+  
+  
+  Notation "'if' c 'then' t 'else' e" :=
+    (CIf c t e) (in custom stimp at level 63): ictree_scope.
+
+  Notation "'if' c 'then' t 'done'" :=
+    (CIf c t CSkip) (in custom stimp at level 63): ictree_scope.
+
+  Notation "'while' c 'do' b 'done'" :=
+    (CWhile c b) (in custom stimp at level 63): ictree_scope.
+
+  Notation "'skip'" :=
+    (CSkip) (in custom stimp at level 63): ictree_scope.
+
+  Notation "t1 ;;; t2" := (CSeq t1 t2) (in custom stimp at level 62, right associativity): stimp_scope.
+  
+  Notation "'var' x '=' c" :=
+    (CNow (vis_with (fun pat : writerE _ =>
+                       let 'Log ctx as z := pat return (encode z -> Prop) in
+                       fun 'tt => lookup x ctx = Some c)))
+      (in custom ticll at level 75): ticl_scope.
+
+  Notation "'var' x '<' c" :=
+    (CNow (vis_with (fun pat : writerE _ =>
+                       let 'Log ctx as z := pat return (encode z -> Prop) in
+                       fun 'tt => exists v, lookup x ctx = Some v /\ v < c)))
+      (in custom ticll at level 75): ticl_scope.
+
+  Notation "'var' x '<=' c" :=
+    (CNow (vis_with (fun pat : writerE _ =>
+                       let 'Log ctx as z := pat return (encode z -> Prop) in
+                       fun 'tt => exists v, lookup x ctx = Some v /\ v <= c)))
+      (in custom ticll at level 75): ticl_scope.
+
+  Notation "'var' x '>' c" :=
+    (CNow (vis_with (fun pat : writerE _ =>
+                       let 'Log ctx as z := pat return (encode z -> Prop) in
+                       fun 'tt => exists v, lookup x ctx = Some v /\ v > c)))
+      (in custom ticll at level 75): ticl_scope.
+
+  Notation "'var' x '>=' c" :=
+    (CNow (vis_with (fun pat : writerE _ =>
+                       let 'Log ctx as z := pat return (encode z -> Prop) in
+                       fun 'tt => exists v, lookup x ctx = Some v /\ v >= c)))
+      (in custom ticll at level 75): ticl_scope.
+  
+  (*| Equality in context |*)
+  Lemma var_eq{X}: forall (p: ictreeW Ctx X) c v m,
+      <( p, {Obs (Log (add c v m)) tt} |= var c = v )>.
+  Proof.
+    intros.
+    apply ticll_vis; constructor.
+    pose proof (mapsto_lookup c v (add c v m)).
+    pose proof (mapsto_add_eq m c v).
+    rewrite <- H in H0.
+    now rewrite H0.
+  Qed.
+
+  Lemma var_neq{X}: forall (p: ictreeW Ctx X) c c' v v' m,
+      <( p, {Obs (Log m) tt} |= var c = v )> ->
+      c <> c' ->
+      <( p, {Obs (Log (add c' v' m)) tt} |= var c = v )>.
+  Proof.
+    intros.
+    apply ticll_vis; constructor.
+    rewrite mapsto_lookup.
+    apply mapsto_add_neq with (R:=eq); eauto. 
+    inv H.
+    dependent destruction H1.
+    apply mapsto_lookup; auto.
+    Unshelve.
+    typeclasses eauto.
+  Qed.
+
+  (*| Less-than-equal in context |*)
+  Lemma var_le{X}: forall (p: ictreeW Ctx X) c v x m,
+      v <= x ->
+      <( p, {Obs (Log (add c v m)) tt} |= var c <= x )>.
+  Proof with auto.
+    intros.
+    apply ticll_vis; constructor.
+    pose proof (mapsto_lookup c v (add c v m)).
+    pose proof (mapsto_add_eq m c v).
+    exists v; split...
+  Qed.
+
+  Lemma var_nle{X}: forall (p: ictreeW Ctx X) c c' v x m,
+      <( p, {Obs (Log m) tt} |= var c <= x )> ->
+      c <> c' ->
+      <( p, {Obs (Log (add c' v m)) tt} |= var c <= x )>.
+  Proof with eauto.
+    intros.
+    apply ticll_vis in H.
+    dependent destruction H.
+    destruct H as (v' & Heq & ?).
+    apply ticll_vis; econstructor.
+    exists v'; split...
+    rewrite mapsto_lookup.
+    apply mapsto_add_neq with (R:=eq); eauto. 
+    apply mapsto_lookup; auto.
+    Unshelve.
+    typeclasses eauto.
+  Qed.
+
+  (*| Less-than in context |*)
+  Lemma var_lt{X}: forall (p: ictreeW Ctx X) c v x m,
+      v < x ->
+      <( p, {Obs (Log (add c v m)) tt} |= var c < x )>.
+  Proof with auto.
+    intros.
+    apply ticll_vis; constructor.
+    pose proof (mapsto_lookup c v (add c v m)).
+    pose proof (mapsto_add_eq m c v).
+    exists v; split...
+  Qed.
+
+  Lemma var_nlt{X}: forall (p: ictreeW Ctx X) c c' v x m,
+      <( p, {Obs (Log m) tt} |= var c < x )> ->
+      c <> c' ->
+      <( p, {Obs (Log (add c' v m)) tt} |= var c < x )>.
+  Proof with eauto.
+    intros.
+    apply ticll_vis in H.
+    dependent destruction H.
+    destruct H as (v' & Heq & ?).
+    apply ticll_vis; econstructor.
+    exists v'; split...
+    rewrite mapsto_lookup.
+    apply mapsto_add_neq with (R:=eq); eauto. 
+    apply mapsto_lookup; auto.
+    Unshelve.
+    typeclasses eauto.
+  Qed.
+
+  (*| Greater-than in context |*)
+  Lemma var_gt{X}: forall (p: ictreeW Ctx X) c v x m,
+      v > x ->
+      <( p, {Obs (Log (add c v m)) tt} |= var c > x )>.
+  Proof with auto.
+    intros.
+    apply ticll_vis; constructor.
+    pose proof (mapsto_lookup c v (add c v m)).
+    pose proof (mapsto_add_eq m c v).
+    exists v; split...
+  Qed.
+
+  Lemma var_ngt{X}: forall (p: ictreeW Ctx X) c c' v x m,
+      <( p, {Obs (Log m) tt} |= var c > x )> ->
+      c <> c' ->
+      <( p, {Obs (Log (add c' v m)) tt} |= var c > x )>.
+  Proof with eauto.
+    intros.
+    apply ticll_vis in H.
+    dependent destruction H.
+    destruct H as (v' & Heq & ?).
+    apply ticll_vis; econstructor.
+    exists v'; split...
+    rewrite mapsto_lookup.
+    apply mapsto_add_neq with (R:=eq); eauto. 
+    apply mapsto_lookup; auto.
+    Unshelve.
+    typeclasses eauto.
+  Qed.
+  
+  (*| Assignment: structural temporal lemmas |*)
+  Lemma aur_cprog_assgn: forall x a ctx r w R ψ,
+      <[ {instr_exp a ctx}, w |= AX done= {(r, ctx)} w ]> ->
+      <( {log (add x r ctx)}, w |= ψ )> ->
+      R (tt, add x r ctx) (Obs (Log (add x r ctx)) tt) ->
+      <[ {instr_prog [[ x := a ]] ctx}, w |= ψ AU AX done R ]>.
+  Proof with eauto with ticl.
+    unfold instr_prog, instr_exp.
+    intros; cbn.
+    eapply aur_state_bind_r_eq.
+    - cleft...
+    - eapply aur_state_bind_r_eq.
+      + eapply aur_get...
+        apply ticll_not_done in H0...
+      + eapply aur_put...
+  Qed.
+  
+  (*| Sequence: structural temporal lemmas |*)
+  Lemma anr_cprog_seq: forall a b ctx ctx' w w' φ ψ,
+      <[ {instr_prog a ctx}, w |= ψ AN done= {(tt,ctx')} w' ]> ->
+      <[ {instr_prog b ctx'}, w' |= ψ AN φ ]> ->
+      <[ {instr_prog [[ a ;;; b ]] ctx}, w |= ψ AN φ ]>.
+  Proof.
+    unfold instr_prog. 
+    intros; cbn.
+    eapply anr_state_bind_r_eq; eauto.
+  Qed.
+  
+  Lemma aur_cprog_seq: forall a b ctx ctx' w w' φ ψ,
+      <[ {instr_prog a ctx}, w |= φ AU AX done= {(tt,ctx')} w' ]> ->
+      <[ {instr_prog b ctx'}, w' |= φ AU ψ ]> ->
+      <[ {instr_prog [[ a ;;; b ]] ctx}, w |= φ AU ψ ]>.
+  Proof.
+    unfold instr_prog.
+    intros; cbn.
+    eapply aur_state_bind_r_eq; eauto.
+  Qed.
+  
+  Lemma aul_cprog_seq: forall a b ctx ctx' w w' φ ψ,
+      <[ {instr_prog a ctx}, w |= φ AU AX done= {(tt,ctx')} w' ]> ->
+      <( {instr_prog b ctx'}, w' |= φ AU ψ )> ->
+      <( {instr_prog [[ a ;;; b ]] ctx}, w |= φ AU ψ )>.
+  Proof.
+    unfold instr_prog. 
+    intros; cbn.
+    eapply aul_state_bind_r_eq; eauto.
+  Qed.
+  
+  Lemma ag_cprog_seq: forall a b ctx ctx' w w' φ,
+      <[ {instr_prog a ctx}, w |= φ AU AX done= {(tt,ctx')} w' ]> ->
+      <( {instr_prog b ctx'}, w' |= AG φ )> ->
+      <( {instr_prog [[ a ;;; b ]] ctx}, w |= AG φ )>.
+  Proof.
+    unfold instr_prog. 
+    intros; cbn.
+    eapply ag_state_bind_r_eq; eauto.
+  Qed.
+
+  (*| Conditional: structural temporal lemmas |*)
+  Lemma aul_cprog_ite: forall c ctx w φ ψ (b: bool) t f,
+      <[ {instr_comp c ctx}, w |= AX done= {(b, ctx)} w ]> ->
+      (if b then
+         <( {instr_prog t ctx}, w |= φ AU ψ )>
+       else
+         <( {instr_prog f ctx}, w |= φ AU ψ )>) ->
+      <( {instr_prog [[ if c then t else f ]] ctx}, w |= φ AU ψ )>.
+  Proof with eauto with ticl.
+    unfold instr_prog, instr_comp. 
+    intros; cbn.
+    eapply aul_state_bind_r_eq.
+    - cleft...
+    - destruct b...
+  Qed.
+
+  Lemma aur_cprog_ite: forall c ctx w φ ψ (b: bool) t f,
+      <[ {instr_comp c ctx}, w |= AX done= {(b, ctx)} w ]> ->
+      (if b then
+         <[ {instr_prog t ctx}, w |= φ AU ψ ]>
+       else
+         <[ {instr_prog f ctx}, w |= φ AU ψ ]>) ->
+      <[ {instr_prog [[ if c then t else f ]] ctx}, w |= φ AU ψ ]>.
+  Proof with eauto with ticl.
+    unfold instr_prog, instr_comp. 
+    intros; cbn.
+    eapply aur_state_bind_r_eq.
+    - cleft...
+    - destruct b...
+  Qed.
+
+  (*| While loops |*)
+  Lemma aul_cprog_while_true: forall c t w w' φ ψ ctx ctx',
+      <[ {instr_comp c ctx}, w |= AX done={(true, ctx)} w ]> ->
+      <[ {instr_prog t ctx}, w |= φ AU AX done={(tt, ctx')} w' ]> ->
+      <( {instr_prog [[ while c do t done ]] ctx'}, w' |= φ AU ψ )> ->   
+      <( {instr_prog [[ while c do t done ]] ctx}, w |= φ AU ψ )>.
+  Proof with eauto with ticl.
+    unfold instr_prog, instr_comp; cbn; intros.
+    apply aul_state_iter_next_eq with tt w' ctx'...
+    - eapply aur_state_bind_r_eq.
+      + cleft...
+      + cbn; apply ticll_not_done in H1.
+        eapply aur_state_bind_r_eq...
+        apply aur_state_ret; intuition.
+    - apply ticll_not_done in H1...
+  Qed.
+
+  Lemma aul_cprog_while_false: forall c t w φ ψ ctx,
+      <[ {instr_comp c ctx}, w |= AX done={(false, ctx)} w ]> ->
+      <( {Ret (tt, ctx)}, w |= ψ )> ->
+      <( {instr_prog [[ while c do t done ]] ctx}, w |= φ AU ψ )>.
+  Proof with eauto with ticl.
+    unfold instr_prog, instr_comp; cbn; intros.
+    rewrite instr_state_unfold_iter.
+    eapply aul_bind_r_eq.
+    - eapply aur_state_bind_r_eq.
+      + cleft...
+      + apply ticll_not_done in H0.
+        apply aur_state_ret...
+    - cleft...
+  Qed.
+
+  Lemma aur_cprog_while_true: forall c t w w' φ ψ ctx ctx',
+      <[ {instr_comp c ctx}, w |= AX done={(true, ctx)} w ]> ->
+      <[ {instr_prog t ctx}, w |= φ AU AX done={(tt, ctx')} w' ]> ->
+      <[ {instr_prog [[ while c do t done ]] ctx'}, w' |= φ AU AX ψ ]> ->   
+      <[ {instr_prog [[ while c do t done ]] ctx}, w |= φ AU AX ψ ]>.
+  Proof with eauto with ticl.
+    unfold instr_prog, instr_comp; cbn; intros.
+    apply aur_state_iter_next_eq with tt w' ctx'...
+    - eapply aur_state_bind_r_eq.
+      + cleft...
+      + cbn. 
+        eapply aur_state_bind_r_eq...
+        apply aur_state_ret; intuition.
+        now apply aur_not_done in H1.
+    - now apply aur_not_done in H1. 
+  Qed.
+
+  Lemma aur_cprog_while_false: forall c t w φ ψ ctx,
+      <[ {instr_comp c ctx}, w |= AX done={(false, ctx)} w ]> ->
+      <[ {Ret (tt, ctx)}, w |= AX ψ ]> ->
+      <[ {instr_prog [[ while c do t done ]] ctx}, w |= φ AU AX ψ ]>.
+  Proof with eauto with ticl.
+    unfold instr_prog, instr_comp; cbn; intros.
+    rewrite instr_state_unfold_iter.
+    eapply aur_bind_r_eq.
+    - eapply aur_state_bind_r_eq.
+      + cleft...
+      + apply aur_state_ret...
+        cdestruct H.
+        apply can_step_not_done in Hs...
+    - cleft...
+  Qed.  
+  
+  (* Termination *)
+  Theorem aur_cprog_while_termination ctx (t: CProg) Ri f w c φ ψ:    
+      not_done w ->
+      Ri ctx ->
+      (forall ctx w (b: bool),
+          not_done w ->
+          Ri ctx ->
+          <[ {instr_comp c ctx}, w |= AX done={(b, ctx)} w ]> /\
+          if b then
+            <[ {instr_prog t ctx}, w |= φ AU AX done {fun '(_, ctx') w' => not_done w' /\ Ri ctx' /\ f ctx' < f ctx} ]>
+          else
+            <[ {Ret (tt, ctx)}, w |= φ AN ψ ]>) ->
+      <[ {instr_prog [[ while c do t done ]] ctx}, w |= φ AU ψ ]>.
+  Proof with eauto with ticl.
+    unfold instr_prog, instr_comp; intros.
+    eapply aur_state_iter_nat with
+      (Ri:=fun 'tt ctx w => exists (b: bool),
+             <[ {instr_stateE (cdenote_comp c) ctx}, w |= AX (done= {(b, ctx)} w) ]> /\
+             if b
+             then
+               <[
+                 {instr_stateE (cdenote_prog t) ctx}, {w}
+                   |= {φ} AU AX (done {fun '(_, ctx') (w' : WorldW Ctx) => not_done w' /\ Ri ctx' /\ f ctx' < f ctx}) ]>
+             else <[ {Ret (tt, ctx)}, {w} |= {φ} AN {ψ} ]>)
+      (f:= fun _ ctx _ => f ctx)...
+    - intros [] ctx' w' Hd ([] & Hb & HR);
+        eapply aur_state_bind_r_eq...
+      + cleft...
+      + eapply aur_state_bind_r.
+        * apply HR.
+        * intros; destruct x.
+          apply aur_state_ret; intuition.
+          exists true...
+      + cleft...
+      + eapply aur_state_ret...
+        Unshelve.
+        exact true.
+  Qed.
+
+  (* Invariance *)
+  Lemma ag_cprog_while: forall c (t: CProg) R ctx w φ,
+      R ctx ->
+      not_done w ->
+      (forall ctx w,
+          R ctx ->
+          not_done w ->
+          <( {instr_prog [[while c do t done ]] ctx}, w |= φ )> /\
+          <[ {instr_comp c ctx}, w |= AX done={(true,ctx)} w ]>  /\            
+          <[ {instr_prog t ctx}, w |= AX (φ AU AX done {fun '(_, ctx') w' => not_done w' /\ R ctx'}) ]>) ->
+    <( {instr_prog [[ while c do t done ]] ctx}, w |= AG φ )>.
+  Proof with eauto with ticl.
+    unfold instr_prog, instr_comp. 
+    intros; subst.
+    eapply ag_state_iter with (R:=fun 'tt ctx w =>
+                                    <( {instr_prog [[while c do t done ]] ctx}, w |= φ )> /\
+                                      <[ {instr_comp c ctx}, w |= AX done={(true,ctx)} w ]>  /\            
+                                      <[ {instr_prog t ctx}, w |= AX (φ AU AX done {fun '(_, ctx') w' => not_done w' /\ R ctx'}) ]>)...
+    - intros [] ctx' w' Hd HR; intuition.
+      rewrite interp_state_bind.
+      eapply anr_bind_r_eq...
+      cbn; rewrite interp_state_bind.
+      cdestruct H5.
+      csplit...      
+      + destruct Hs as (t_ & w_ & TR).
+        eapply can_step_bind_l...
+        specialize (H5 _ _ TR).
+        now apply aur_not_done in H5.
+      + intros t_ w_ TR...
+        apply ktrans_bind_inv in TR as [(? & TR & Hd_ & ->) | (([] & ctx_) & ? & ? & ? & TR)].
+        * specialize (H5 _ _ TR).
+          apply aur_bind_r with (R:=fun '(_, ctx') (w' : WorldW Ctx) => not_done w' /\ R ctx')...
+          intros [_ ctx_] w'' (Hd'' & HR').
+          apply aur_state_ret...
+        * specialize (H5 _ _ H3).
+          now apply aur_stuck, anr_stuck in H5.
+  Qed.
+  
+End StImp.
